Added an easy to user parser for "Circus-M"

tutorial/utp_csp_buffer.thy
@@ -1,7 +1,7 @@
 section \<open> Simple Buffer in UTP CSP \<close>
 
 theory utp_csp_buffer
-  imports "UTP-Circus.utp_circus"
+  imports "UTP-Circus.utp_circus_easy_parser"
 begin
 
 subsection \<open> Definitions \<close>
@@ -13,6 +13,7 @@ text \<open> A stateful CSP (Circus) process is parametrised over two alphabets:
 
 alphabet st_buffer =
   buff :: "nat list"
+  val  :: "nat"
 
 text \<open> Channels are created using the \textbf{datatype} command. In this case we can either input
   a value to go in the buffer, or output one presently in the buffer. \<close>
@@ -28,21 +29,21 @@ type_synonym act_buffer = "(st_buffer, ch_buffer) action"
 text \<open> We define an action that initialises the buffer state by setting it to empty. \<close>
 
 abbreviation Init :: act_buffer where
-"Init \<equiv> buff :=\<^sub>C \<langle>\<rangle>"
+"Init \<equiv> buff := []"
 
 text \<open> We define the main body of behaviour for the buffer as an abbreviation. We can either
   input a value and then place it into the buffer, or else, provided that the buffer is non-empty,
   we can output a value presently in the buffer. \<close>
 
 abbreviation DoBuff :: act_buffer where
-"DoBuff \<equiv> (inp?(v) \<^bold>\<rightarrow> buff :=\<^sub>C &buff ^\<^sub>u \<langle>\<guillemotleft>v\<guillemotright>\<rangle>
-           \<box> (#\<^sub>u(&buff) >\<^sub>u 0) &\<^sub>u outp!(head\<^sub>u(&buff)) \<^bold>\<rightarrow> buff :=\<^sub>C tail\<^sub>u(&buff))"
+"DoBuff \<equiv> (inp?(val) ;; buff := buff @ [val]
+           \<box> #buff > 0 && outp!(hd(buff)) ;; buff := tl(buff))"
 
 text \<open> The main action of the buffer first initialises the single state variable $buff$, and
   enters a recursive loop where it does \emph{DoBuff} over and over. \<close>
 
 definition Buffer :: act_buffer where
-[rdes_def]: "Buffer = Init ;; while\<^sub>R true do DoBuff od"
+[rdes_def]: "Buffer = Init ;; while true do DoBuff od"
 
 subsection \<open> Calculations \<close>
 
@@ -58,13 +59,13 @@ lemma Init_contract:
 lemma DoBuff_contract:
   "DoBuff = \<^bold>R\<^sub>s (true\<^sub>r \<turnstile>
                 \<E>(true,\<langle>\<rangle>, (\<Sqinter> x \<bullet> {(inp\<cdot>\<guillemotleft>x\<guillemotright>)\<^sub>u}\<^sub>u) \<union>\<^sub>u ({(outp\<cdot>head\<^sub>u(&buff))\<^sub>u}\<^sub>u \<triangleleft> 0 <\<^sub>u #\<^sub>u(&buff) \<triangleright> {}\<^sub>u)) \<diamondop>
-                ((\<Sqinter> x \<bullet> \<Phi>(true,[&buff \<mapsto>\<^sub>s &buff ^\<^sub>u \<langle>\<guillemotleft>x\<guillemotright>\<rangle>],\<langle>(inp\<cdot>\<guillemotleft>x\<guillemotright>)\<^sub>u\<rangle>)) \<or>
+                ((\<Sqinter> x \<bullet> \<Phi>(true,[&buff \<mapsto>\<^sub>s &buff ^\<^sub>u \<langle>\<guillemotleft>x\<guillemotright>\<rangle>, val \<mapsto>\<^sub>s \<guillemotleft>x\<guillemotright>],\<langle>(inp\<cdot>\<guillemotleft>x\<guillemotright>)\<^sub>u\<rangle>)) \<or>
                  \<Phi>(0 <\<^sub>u #\<^sub>u(&buff), [&buff \<mapsto>\<^sub>s tail\<^sub>u(&buff)], \<langle>(outp\<cdot>head\<^sub>u(&buff))\<^sub>u\<rangle>)))"
   by (rdes_eq)
 
 lemma Buffer_contract:
   "Buffer = \<^bold>R\<^sub>s(true\<^sub>r \<turnstile> \<Phi>(true,[&buff \<mapsto>\<^sub>s \<langle>\<rangle>],\<langle>\<rangle>) ;;
-                       ((\<Sqinter> x \<bullet> \<Phi>(true, [&buff \<mapsto>\<^sub>s &buff ^\<^sub>u \<langle>\<guillemotleft>x\<guillemotright>\<rangle>], \<langle>(inp\<cdot>\<guillemotleft>x\<guillemotright>)\<^sub>u\<rangle>)) \<or>
+                       ((\<Sqinter> x \<bullet> \<Phi>(true, [&buff \<mapsto>\<^sub>s &buff ^\<^sub>u \<langle>\<guillemotleft>x\<guillemotright>\<rangle>, val \<mapsto>\<^sub>s \<guillemotleft>x\<guillemotright>], \<langle>(inp\<cdot>\<guillemotleft>x\<guillemotright>)\<^sub>u\<rangle>)) \<or>
                         \<Phi>(0 <\<^sub>u #\<^sub>u(&buff), [&buff \<mapsto>\<^sub>s tail\<^sub>u(&buff)], \<langle>(outp\<cdot>head\<^sub>u(&buff))\<^sub>u\<rangle>))\<^sup>\<star>\<^sup>r ;;
                         \<E>(true,\<langle>\<rangle>, (\<Sqinter> x \<bullet> {(inp\<cdot>\<guillemotleft>x\<guillemotright>)\<^sub>u}\<^sub>u) \<union>\<^sub>u ({(outp\<cdot>head\<^sub>u(&buff))\<^sub>u}\<^sub>u \<triangleleft> 0 <\<^sub>u #\<^sub>u(&buff) \<triangleright> {}\<^sub>u)) \<diamondop>
                        false)"
@@ -78,8 +79,7 @@ abbreviation "inps t \<equiv> [x. inp x \<leftarrow> t]"
 abbreviation "outps t \<equiv> [x. outp x \<leftarrow> t]"
 
 lemma P1_lemma:
-  "[true \<turnstile> \<guillemotleft>outps(trace)\<guillemotright> \<le>\<^sub>u &buff ^\<^sub>u \<guillemotleft>inps(trace)\<guillemotright> | true]\<^sub>C \<sqsubseteq> while\<^sub>R true do DoBuff od"
-  apply (simp add: closure)
+  "[true \<turnstile> (outps(\<guillemotleft>trace\<guillemotright>) \<le> (buff @ inps(\<guillemotleft>trace\<guillemotright>))) | true]\<^sub>C \<sqsubseteq> while\<^sub>R true do DoBuff od"
   apply (rdes_refine_split)
     apply (simp_all add: rpred closure usubst)
   apply (rule conjI)
@@ -97,14 +97,22 @@ lemma P1_lemma:
     apply (smt Prefix_Order.Cons_prefix_Cons append.left_neutral append_Cons ch_buffer.simps(6) concat_map_maps hd_Cons_tl less_eq_list_def maps_simps(1) prefix_code(2))
 done 
 
-lemma P1: "[true \<turnstile> \<guillemotleft>outps(trace)\<guillemotright> \<le>\<^sub>u \<guillemotleft>inps(trace)\<guillemotright> | true]\<^sub>C \<sqsubseteq> Buffer"
+lemma P1: "[true \<turnstile> outps(\<guillemotleft>trace\<guillemotright>) \<le> inps(\<guillemotleft>trace\<guillemotright>) | true]\<^sub>C \<sqsubseteq> Buffer"
 proof -
-  have "[true \<turnstile> \<guillemotleft>outps(trace)\<guillemotright> \<le>\<^sub>u \<guillemotleft>inps(trace)\<guillemotright> | true]\<^sub>C
+  have "[true \<turnstile> outps(\<guillemotleft>trace\<guillemotright>) \<le> inps(\<guillemotleft>trace\<guillemotright>) | true]\<^sub>C
         \<sqsubseteq>
-        Init ;; [true \<turnstile> \<guillemotleft>outps(trace)\<guillemotright> \<le>\<^sub>u &buff ^\<^sub>u \<guillemotleft>inps(trace)\<guillemotright> | true]\<^sub>C"
+        Init ;; [true \<turnstile> outps(\<guillemotleft>trace\<guillemotright>) \<le> inps(\<guillemotleft>trace\<guillemotright>) | true]\<^sub>C"
     by (rdes_refine)
-  thus ?thesis
-    by (metis (no_types, lifting) Buffer_def P1_lemma dual_order.trans urel_dioid.mult_isol)
+  moreover have "Init ;; [true \<turnstile> outps(\<guillemotleft>trace\<guillemotright>) \<le> inps(\<guillemotleft>trace\<guillemotright>) | true]\<^sub>C 
+                 \<sqsubseteq>
+                 Init ;; [true \<turnstile> outps(\<guillemotleft>trace\<guillemotright>) \<le> (buff @ inps(\<guillemotleft>trace\<guillemotright>)) | true]\<^sub>C"
+    by (rdes_refine)
+  moreover have "Init ;; [true \<turnstile> outps(\<guillemotleft>trace\<guillemotright>) \<le> (buff @ inps(\<guillemotleft>trace\<guillemotright>)) | true]\<^sub>C
+                 \<sqsubseteq>
+                 Buffer"
+    by (simp add: Buffer_def P1_lemma urel_dioid.mult_isol)
+  ultimately show ?thesis
+    by (simp)
 qed
 
 lemma Buffer_deadlock_free: "CDF \<sqsubseteq> Buffer"
